theories/serialization/SerializeConfig.v
@@ -113,6 +113,24 @@ Instance Serialize_cakeml_config' : Serialize cakeml_config' :=
   fun o =>
     @to_sexp _ Serialize_unit o.
 
+Instance Serialize_catcrypt_config : Serialize catcrypt_config :=
+  fun o =>
+    [Atom "catcrypt_config";
+     to_sexp (catcrypt_namespace o);
+     to_sexp (catcrypt_def_name o);
+     to_sexp (catcrypt_mask63 o);
+     to_sexp (catcrypt_scaffold o)
+    ]%sexp.
+
+Instance Serialize_catcrypt_config' : Serialize catcrypt_config' :=
+  fun o =>
+    [Atom "catcrypt_config";
+     to_sexp (catcrypt_namespace' o);
+     to_sexp (catcrypt_def_name' o);
+     to_sexp (catcrypt_mask63' o);
+     to_sexp (catcrypt_scaffold' o)
+    ]%sexp.
+
 Instance Serialize_eval_config : Serialize eval_config :=
   fun o =>
     [Atom "eval_config";
@@ -172,6 +190,7 @@ Instance Serialize_backend_config : Serialize backend_config :=
     | Wasm o => [Atom "Wasm"; to_sexp o ]
     | OCaml o => [Atom "OCaml"; to_sexp o ]
     | CakeML o => [Atom "CakeML"; to_sexp o ]
+    | CatCrypt o => [Atom "CatCrypt"; to_sexp o ]
     | Eval o => [Atom "Eval"; to_sexp o ]
     | AST o => [Atom "AST"; to_sexp o ]
     end%sexp.
@@ -185,6 +204,7 @@ Instance Serialize_backend_config' : Serialize backend_config' :=
     | Wasm' o => [Atom "Wasm"; to_sexp o ]
     | OCaml' o => [Atom "OCaml"; to_sexp o ]
     | CakeML' o => [Atom "CakeML"; to_sexp o ]
+    | CatCrypt' o => [Atom "CatCrypt"; to_sexp o ]
     | Eval' o => [Atom "Eval"; to_sexp o ]
     | AST' o => [Atom "AST"; to_sexp o ]
     end%sexp.
@@ -350,6 +370,12 @@ Definition string_of_cakeml_config (x : cakeml_config) : string :=
 
 Definition string_of_cakeml_config' (x : cakeml_config') : string :=
   @to_string cakeml_config' Serialize_cakeml_config' x.
+
+Definition string_of_catcrypt_config (x : catcrypt_config) : string :=
+  @to_string catcrypt_config Serialize_catcrypt_config x.
+
+Definition string_of_catcrypt_config' (x : catcrypt_config') : string :=
+  @to_string catcrypt_config' Serialize_catcrypt_config' x.
 
 Definition string_of_eval_config (x : eval_config) : string :=
   @to_string eval_config Serialize_eval_config x.
